while total
git-svn-id: orca@452

C-verifier/src/Midend-IVL/Isabelle-UTP-Extended/utp/utp_rec_total.thy
@@ -129,7 +129,37 @@ lemma total_rec_test:
       apply (rule prems(2))  
       using prems(1) apply pred_simp 
       done
-done
- 
+    done
+      
+definition while_invT :: "'\<alpha> cond \<Rightarrow> '\<alpha> cond \<Rightarrow> '\<alpha> hrel \<Rightarrow> '\<alpha> hrel" ("while\<^sub>\<bottom> _ invr _ do _ od" 71) where
+"while\<^sub>\<bottom> b invr p do S od = while\<^sub>\<bottom> b do S od"  
+
+
+lemma uwhile_total_rule:
+  assumes WF: "wf R"
+  assumes I0: "`Pre \<Rightarrow> I`"
+  assumes induct_step:"\<And> st. (\<lceil>b \<and> I \<and>  E =\<^sub>u \<guillemotleft>st\<guillemotright> \<rceil>\<^sub>< \<Rightarrow> (\<lceil>I \<and>(E,\<guillemotleft>st\<guillemotright>)\<^sub>u\<in>\<^sub>u\<guillemotleft>R\<guillemotright> \<rceil>\<^sub>> )) \<sqsubseteq> f"  
+  assumes PHI:"`\<not> \<lceil>b\<rceil>\<^sub>< \<and> \<lceil>I\<rceil>\<^sub>< \<Rightarrow> \<lceil>Post\<rceil>\<^sub>>`"  
+  shows "\<lbrace>Pre\<rbrace>while\<^sub>\<bottom> b invr I do f od\<lbrace> Post\<rbrace>\<^sub>u"
+  unfolding  hoare_r_def while_invT_def while_bot_def
+   apply (rule pre_weak_rel[of _ "\<lceil>I\<rceil>\<^sub><" ])
+  using I0 
+   apply pred_simp
+    apply (rule rec_total_utp_rule[where Pre="\<lceil>I\<rceil>\<^sub><" and E = E, OF WF])  
+   apply (simp add: cond_mono monoI seqr_mono)
+  apply (rule  cond_refine_rel)
+     prefer 2
+   apply (rule skip_refine_rel)
+  using PHI
+   apply pred_blast
+    subgoal for  st 
+      apply (rule_tac seq_refine_unrest[where s= "I \<and> (E,\<guillemotleft>st\<guillemotright>)\<^sub>u\<in>\<^sub>u\<guillemotleft>R\<guillemotright>" ])
+         apply pred_simp
+        apply pred_simp
+       apply (rule order_trans[OF induct_step, where st1 = st]) 
+       apply pred_simp 
+      apply pred_simp
+done        
+  done 
 
 end
