C-verifier/src/Backend/VCG/VCG_rel_Floyd.thy
@@ -1,6 +1,6 @@
 section \<open>VCG for total correctness using Floyd assignment\<close>
 
-theory VCG_rel_Floyd
+theory VCG_rel_Floyd                                           
   imports "../../Midend-IVL/Isabelle-UTP-Extended/hoare/HoareLogic/PartialCorrectness/utp_hoare"
 begin
 
