C-verifier/src/Midend-IVL/Isabelle-UTP-Extended/utp/utp_rec_total_des.thy
@@ -1,39 +1,39 @@
 theory utp_rec_total_des
   imports "../../Isabelle-UTP/theories/utp_designs"
 begin
-
-lemma  wf_fixp_uinduct_desr: 
+  
+lemma  wf_fixp_induct_pure_des_rule: 
   assumes fixp_unfold: "fp B = B (fp B)"
   and              WF: "wf R"
   and     induct_step:
-          "\<And> f st. (\<forall>st'. ((st',st) \<in>R  \<longrightarrow> ((Pre \<turnstile>\<^sub>r Post)\<lbrakk>\<guillemotleft>st'\<guillemotright>/$\<Sigma>\<rbrakk> \<sqsubseteq> f\<lbrakk>\<guillemotleft>st'\<guillemotright>/$\<Sigma>\<rbrakk>))
-               \<Longrightarrow> fp B = f \<Longrightarrow>(Pre \<turnstile>\<^sub>r Post)\<lbrakk>\<guillemotleft>st\<guillemotright>/$\<Sigma>\<rbrakk> \<sqsubseteq> (B f)\<lbrakk>\<guillemotleft>st\<guillemotright>/$\<Sigma>\<rbrakk>)"
-        shows "((Pre \<turnstile>\<^sub>r Post) \<sqsubseteq> fp B)"  
-proof -
-  { fix st 
-    have "((Pre \<turnstile>\<^sub>r Post)\<lbrakk>\<guillemotleft>st\<guillemotright>/$\<Sigma>\<rbrakk> \<sqsubseteq> (fp B)\<lbrakk>\<guillemotleft>st\<guillemotright>/$\<Sigma>\<rbrakk>)" 
-      using WF
-      apply (induction st rule: wf_induct_rule)  
-      apply (subst fixp_unfold)  
-      apply (rule induct_step)  
-      apply blast
-      apply simp  
-      done  
-  }
-  thus ?thesis
-    by rel_auto
-qed
-
-lemma  wf_fixp_uinduct_des: 
-  assumes fixp_unfold: "fp B = B (fp B)"
-  and              WF: "wf R"
-  and     induct_step:
-          "\<And>f st. (\<forall>st'. ((st',st) \<in>R  \<longrightarrow> ((Pre \<turnstile> Post)\<lbrakk>\<guillemotleft>st'\<guillemotright>/$\<Sigma>\<rbrakk> \<sqsubseteq> f\<lbrakk>\<guillemotleft>st'\<guillemotright>/$\<Sigma>\<rbrakk>))
-               \<Longrightarrow> fp B = f \<Longrightarrow>(Pre \<turnstile> Post)\<lbrakk>\<guillemotleft>st\<guillemotright>/$\<Sigma>\<rbrakk> \<sqsubseteq> (B f)\<lbrakk>\<guillemotleft>st\<guillemotright>/$\<Sigma>\<rbrakk>)"
+          "\<And>f st. \<lbrakk>\<And>st'. (st',st) \<in> R  \<Longrightarrow> (((Pre \<and> \<lceil>E\<rceil>\<^sub><  =\<^sub>u\<guillemotleft>st'\<guillemotright>) \<turnstile> Post) \<sqsubseteq> f)\<rbrakk> \<Longrightarrow> 
+           fp B = f \<Longrightarrow>((Pre \<and> \<lceil>E\<rceil>\<^sub><  =\<^sub>u \<guillemotleft>st\<guillemotright>) \<turnstile> Post) \<sqsubseteq> (B f)"
   shows "((Pre \<turnstile> Post) \<sqsubseteq> fp B)"  
 proof -
   { fix st 
-    have "((Pre \<turnstile> Post)\<lbrakk>\<guillemotleft>st\<guillemotright>/ $\<Sigma>\<rbrakk> \<sqsubseteq> (fp B)\<lbrakk>\<guillemotleft>st\<guillemotright>/$\<Sigma>\<rbrakk>)" 
+    have "(((Pre \<and> \<lceil>E\<rceil>\<^sub><  =\<^sub>u \<guillemotleft>st\<guillemotright>) \<turnstile> Post) \<sqsubseteq> (fp B))" 
+      using WF
+      apply (induction st rule: wf_induct_rule)  
+      apply (subst fixp_unfold)  
+      apply (rule induct_step)  
+      apply blast
+      apply simp  
+      done  
+  }
+  thus ?thesis
+    by rel_auto
+qed  
+  
+lemma  wf_fixp_induct_pure_desr_rule: 
+  assumes fixp_unfold: "fp B = B (fp B)"
+  and              WF: "wf R"
+  and     induct_step:
+          "\<And> f st. \<lbrakk>\<And>st'. ((st',st) \<in> R  \<Longrightarrow> ((Pre \<and> \<lceil>E\<rceil>\<^sub>< =\<^sub>u\<guillemotleft>st'\<guillemotright>) \<turnstile>\<^sub>r Post) \<sqsubseteq> f)\<rbrakk> \<Longrightarrow> 
+           fp B = f \<Longrightarrow>((Pre \<and> \<lceil>E\<rceil>\<^sub><  =\<^sub>u\<guillemotleft>st\<guillemotright>) \<turnstile>\<^sub>r Post) \<sqsubseteq> (B f)"
+        shows "(Pre \<turnstile>\<^sub>r Post) \<sqsubseteq> fp B"  
+proof -
+  { fix st 
+    have "((Pre \<and> \<lceil>E\<rceil>\<^sub><  =\<^sub>u\<guillemotleft>st\<guillemotright>) \<turnstile>\<^sub>r Post) \<sqsubseteq> (fp B)" 
       using WF
       apply (induction st rule: wf_induct_rule)  
       apply (subst fixp_unfold)  
@@ -45,6 +45,7 @@ proof -
   thus ?thesis
     by rel_auto
 qed
+
 
 lemma  rec_total_rule_des: 
   assumes WF: "wf R"
