C-verifier/README.txt
@@ -1,6 +1,6 @@
 The folder src contains the *.thy theories for the formalization of C semantics.
 
-The set of *.thy files provides a formal framework for implementing imperative programs ins general and C programs in particular.
+The set of *.thy files provides a formal framework for implementing imperative programs in general and C programs in particular.
 
 The framework follows the terminology and the methodology of the informal language IMP, presented in the textbook of Glynn Winskel.
 
